specification/Statics.v
@@ -3,14 +3,48 @@ Require Import List.
 Import ListNotations.
 Require Import Dynamics.
 
-Inductive ty :=
+Inductive ty := 
   | Pub
   | Middle
   | Sec.
 
 Scheme Equality for ty.
 
-Definition max (t1 : ty) (t2 : ty) :=
+Record Lattice := {
+    carrier : Set;
+    le : carrier -> carrier -> bool;
+    max : carrier -> carrier -> carrier;
+    bot : carrier;
+    bot_le : forall x, le bot x = true;
+    refl_le : forall t, le t t = true;
+    assym_le : forall t1 t2, le t1 t2 = true -> le t2 t1 = true -> t1 = t2
+}.
+
+Section Types.
+  Variable (L : Lattice).
+
+Definition context : Type := list (string *  (L.(carrier))). 
+
+Inductive has_type : context -> tm -> L.(carrier) -> Prop :=
+| T_Var : forall Gamma x t1,
+    lookup Gamma x = Some t1 ->
+    has_type Gamma (tm_var x) t1
+| T_Val : forall Gamma v,
+    has_type Gamma (tm_val v) L.(bot)
+| T_Un : forall Gamma e t,
+    has_type Gamma e t ->
+    has_type Gamma (tm_un e) t
+| T_Bin : forall Gamma e1 e2 t1 t2,
+    has_type Gamma e1 t1 ->
+    has_type Gamma e2 t2 ->
+    has_type Gamma (tm_bin e1 e2) (L.(max) t1 t2)
+| T_Let : forall Gamma e1 e2 x t1 t2,
+    has_type Gamma e1 t1 ->
+    has_type (update Gamma x t1) e2 t2 ->
+    has_type Gamma (tm_let x e1 e2) t2.
+
+
+Definition base_max (t1 : ty) (t2 : ty) :=
   match t1, t2 with
   | Pub, Pub => Pub
   | Sec, Sec => Sec
@@ -23,7 +57,7 @@ Definition max (t1 : ty) (t2 : ty) :=
   | Sec, Pub => Sec
   end.
 
-Definition le (t1 t2 : ty) :=
+Definition base_le (t1 t2 : ty) :=
 match t1, t2 with
   | Pub, Pub => true
   | Sec, Sec => true
@@ -34,63 +68,49 @@ match t1, t2 with
   | _ , _ => false
   end.
 
-Lemma le_reflexive (t: ty):
-  le t t = true.
+Lemma base_bot_le (t : ty):
+  base_le Pub t = true.
+Proof.
+  destruct t; simpl; auto.
+Qed.
+
+
+Lemma base_le_reflexive (t: ty):
+  base_le t t = true.
 Proof.
   destruct t; simpl; reflexivity.
 Qed.
 
-Lemma le_assym (t1 t2 : ty):
-  le t1 t2 = true -> le t2 t1 = true -> t1 = t2.
+Lemma base_le_assym (t1 t2 : ty):
+  base_le t1 t2 = true -> base_le t2 t1 = true -> t1 = t2.
 Proof.
 intros h1 h2.
 destruct t1; destruct t2; auto; discriminate.
 Qed.
 
-Lemma le_trans (t1 t2 t3: ty) :
-  le t1 t2 = true -> le t2 t3 = true -> le t1 t3 = true.
+Lemma base_le_trans (t1 t2 t3: ty) :
+  base_le t1 t2 = true -> base_le t2 t3 = true -> base_le t1 t3 = true.
 Proof.
 intros h1 h2.
 destruct t1; destruct t2; destruct t3; auto.
 Qed.
 
-Lemma le_max_eq (t1 t2 : ty) : 
-  le t1 t2 = true ->
-  max t1 t2 = t2.
+Lemma base_le_max_eq (t1 t2 : ty) : 
+  base_le t1 t2 = true ->
+  base_max t1 t2 = t2.
 Proof.
 intros h1.
 destruct t1; destruct t2; simpl; auto; discriminate.
 Qed.
 
-Definition context : Type := list (string * ty).
+Definition base_lattice := {|
+  carrier := ty;
+  le := base_le;
+  max := base_max;
+  bot := Pub;
+  bot_le := base_bot_le;
+  refl_le := base_le_reflexive;
+  assym_le := base_le_assym |}.
 
-Inductive has_type : context -> tm -> ty -> Prop :=
-| T_Var : forall Gamma x t1,
-    lookup Gamma x = Some t1 ->
-    has_type Gamma (tm_var x) t1
-| T_Val : forall Gamma v,
-    has_type Gamma (tm_val v) Pub
-| T_Un : forall Gamma e t,
-    has_type Gamma e t ->
-    has_type Gamma (tm_un e) t
-| T_Bin : forall Gamma e1 e2 t1 t2,
-    has_type Gamma e1 t1 ->
-    has_type Gamma e2 t2 ->
-    has_type Gamma (tm_bin e1 e2) (max t1 t2)
-| T_Let : forall Gamma e1 e2 x t1 t2,
-    has_type Gamma e1 t1 ->
-    has_type (update Gamma x t1) e2 t2 ->
-    has_type Gamma (tm_let x e1 e2) t2.
-    
-
-(*
-Idea: generalize type_rel to have type ty -> ty -> nat -> nat -> Prop.
-(pretty much done!)
-First argument: o : "observer label"
-    - If t <= o, then type_rel o t v1 v2
-    - Otherwise: type_rel o t1 v1 v2 <-> old_type_rel Sec v1 v2
-*)
-
-
-    
+  End Types.
     
